\section{Resumen de propiedades}

\begin{enumerate}
 \item { $ \sum_{i=1}^n{c. a_i}= c \times \sum_{i=1}^n{ a_i}$ \newline \newline Ejemplo: $\sum_{i=1}^{73}{5i}= 5 \times \sum_{i=1}^{73}{ i}$ }
 \item { $\sum_{i=1}^n{c}=(n-1+1) \times c= n \times c$ \newline \newline Ejemplo: $\sum_{i=7}^{19}{cte} = (19-7+1) \times cte = 13 \times cte$ }
 \item { $\sum_{i=1}^n{a_i+b_i}=\sum_{i=1}^n{ a_i} + \sum_{i=1}^n{b_i}$ \newline \newline Ejemplo: $\sum_{i=1}^n{i+3i^2} =\sum_{i=1}^n{i} + \sum_{i=1}^n{3i^2}$ }
 \item { $\sum_{i=1}^n{a_i}=\sum_{i=1}^k{a_i} + \sum_{i=k+1}^n{a_i}$ \newline \newline Ejemplo: $ \sum_{i=1}^n{3i^2} =\sum_{i=1}^5{3i^2} + \sum_{i=6}^n{3i^2} $}
 \item { $\sum_{i=k}^n{a_i}=\sum_{i=1}^n{a_i} - \sum_{i=1}^{k-1}{a_i} $ \newline \newline Ejemplo: $  \sum_{i=7}^{51}{(cte.i+3)} = \sum_{i=1}^{51}{(cte.i+3)} - \sum_{i=1}^{50}{(cte.i+3)} $}
 \item { $\sum_{i=1}^n{a_i \times b_i} \not= \sum_{i=1}^n{ a_i} \times \sum_{i=1}^n{b_i} $ }
 \item { $\sum_{i=1}^n{a_i^2} \not= (\sum_{i=1}^n{ a_i})^2$ }
\end{enumerate}
